thys/core_pre.thy
@@ -1,14 +1,25 @@
+section {* Language Primitives *}
+
 theory core_pre
-imports Main "~~/src/HOL/Library/While_Combinator"
+imports
+  Main
+  "~~/src/HOL/Word/Word"
+  "~~/src/HOL/Library/While_Combinator"
 begin
+
+subsection {* Control Flow *}
+
+subsubsection {* Succinct Monadic Bind Notation *}
 
 nonterminal dobinds and dobind
 syntax
   "_bind"       :: "[pttrn, 'a] => dobind"              ("(2_ \<leftarrow>/ _)" 10)
-  "_Do"         :: "[dobind, 'a] => 'a"                 ("(do (_)/; (_))" [0, 10] 10)
+  "_Do"         :: "[dobind, 'a] => 'a"                 ("(do (_);/ (_))" [0, 10] 10)
 
 translations
   "do x \<leftarrow> a; e"        == "CONST Option.bind a (%x. e)"
+
+subsubsection {* Generalized While Combinator *}
 
 definition loop :: "('state \<Rightarrow> 'state \<times> bool) \<Rightarrow> 'state \<Rightarrow> 'state option" where
   "loop l s \<equiv> map_option (\<lambda>(s,s',c). s')
@@ -24,12 +35,69 @@ definition loop' :: "('state \<Rightarrow> ('state \<times> bool) option) \<Righ
     (Some s)
   ) id"
 
-type_synonym u32 = nat
-type_synonym usize = nat
+subsection {* Types *}
 
-definition[simp]: "u32_to_usize = id"
+subsubsection {* Machine Types *}
 
-definition[simp]: "core_num_u32_overflowing_add x y = Some (x + y, False)"
+type_synonym u8 = "8 word"
+type_synonym u16 = "16 word"
+type_synonym u32 = "32 word"
+type_synonym u64 = "64 word"
+
+abbreviation "u8 n \<equiv> word_of_int n::u8"
+abbreviation "u16 n \<equiv> word_of_int n::u16"
+abbreviation "u32 n \<equiv> word_of_int n::u32"
+abbreviation "u64 n \<equiv> word_of_int n::u64"
+
+lift_definition uint_with_overflow :: "(int \<Rightarrow> int \<Rightarrow> int) \<Rightarrow> 'a::len0 word \<Rightarrow> 'a word \<Rightarrow> 'a word \<times> bool" is "\<lambda>f n m.
+  let i = f (uint n) (uint m)in
+  (i, uint (word_of_int i::'a word) \<noteq> i)" .
+
+lift_definition uint_checked :: "(int \<Rightarrow> int \<Rightarrow> int) \<Rightarrow> 'a::len0 word \<Rightarrow> 'a word \<Rightarrow> 'a word option" is "\<lambda>f n m. case uint_with_overflow f n m of
+  (n, False) \<Rightarrow> Some n
+| (_, True)  \<Rightarrow> None" .
+
+abbreviation "checked_add \<equiv> uint_checked (op +)"
+abbreviation "checked_sub \<equiv> uint_checked (op -)"
+abbreviation "checked_mul \<equiv> uint_checked (op *)"
+abbreviation "checked_div \<equiv> uint_checked (op div)"
+abbreviation "checked_mod \<equiv> uint_checked (op mod)"
+
+subsubsection {* Machine-Dependent Integer Types *}
+
+consts native_bs :: nat
+
+(* let's be somewhat realistic *)
+specification (native_bs) native_bs_min: "native_bs \<ge> 32"
+by auto
+
+typedef native_bs = "UNIV :: unit set" ..
+
+instantiation native_bs :: len
+begin
+  definition "len_of_native_bs (_ :: native_bs itself) = native_bs"
+
+  instance 
+  using native_bs_min
+  by intro_classes (simp add: len_of_native_bs_def)
+end
+
+type_synonym usize = "native_bs word"
+
+abbreviation "usize n \<equiv> word_of_int n::usize"
+
+subsubsection {* Manually-Translated Types *}
+
+typedef 'a slice = "{xs::'a list. length xs < 2^native_bs}"
+by (rule exI[where x="[]"], simp)
+
+subsection {* Functions *}
+
+subsubsection {* Intrinsics *}
+
+abbreviation "core_intrinsics_add_with_overflow n m \<equiv> Some (uint_with_overflow (op +) n m)"
+
+subsubsection {* Manually-Translated Functions *}
 
 definition[simp]: "core_mem_swap x y = Some ((),y,x)"
 
