thys/examples.thy
@@ -2,17 +2,78 @@ theory examples
 imports core examples_export Binomial
 begin
 
-lemma fac: "examples_fac n = Some (fact n)"
-apply simp
-apply (rule loop_range_u32'[where P="\<lambda>i res. res = fact (i-1)"])
-   apply (auto simp: examples_fac_4_def)[1]
-  apply clarsimp
-proof-
-  show "fact (max (Suc 0) n) = fact n"
-  by (cases n; auto)
-
-  show "\<And>i res. 2 \<le> i \<Longrightarrow> res = fact (i - 1) \<Longrightarrow> res * i = fact (Suc i - 1)"
-  by (case_tac i; auto)
+lemma fact_greater_arg: "n > 2 \<Longrightarrow> n < fact n"
+proof (induction n)
+  case (Suc n)
+  show ?case
+  proof (cases "n > 2")
+    case False
+    with Suc show ?thesis
+    apply (cases n)
+     apply simp
+    apply (rename_tac pn)
+    apply (case_tac pn)
+    by auto
+  next
+    case True
+    hence "Suc n < n + n" by simp
+    also have "\<dots> \<le> fact n + n" using True Suc by simp
+    also have "\<dots> \<le> fact (Suc n)" by simp
+    finally show ?thesis by simp
+  qed
 qed simp
+
+declare semiring_numeral_class.power_numeral [simp del]
+
+lemma fac:
+  assumes "fact n < (2::int)^32"
+  shows "examples_fac (u32 (int n)) = Some (u32 (fact n))"
+proof-
+  have [simp]: "Suc n < 2^32"
+    using fact_greater_arg[of n] assms
+    by (cases "n > 2") auto
+
+  have 0: "\<And>i. i > 0 \<Longrightarrow> fact (i - Suc 0) * int i = fact i"
+    by (case_tac i; auto)
+
+  have 1: "\<And>i. i > 0 \<Longrightarrow> fact (nat i - Suc 0) * i = fact (nat i)"
+    by (case_tac i; simp add: 0)
+
+  have 3: "\<And>i. i < u32 (int n) + 1 \<Longrightarrow> unat i < n"
+    sorry
+
+  have [simp]: "\<And>(i::u32) j. 2 \<le> i \<Longrightarrow> i < j \<Longrightarrow> unat (i + 1) - Suc 0 = unat i"
+    by unat_arith
+
+  have 3: "\<And>i. 2 \<le> i \<Longrightarrow> i < u32 (int n) + 1 \<Longrightarrow> fact (unat i-1) < (2::int)^32 \<Longrightarrow> fact (unat i) < (2::int)^32"
+  apply (rule less_trans[of _ "fact n"])
+   apply (rule fact_less_mono)
+    apply unat_arith
+   apply (erule 3)
+  using assms
+  apply simp
+  done
+
+  have 2: "\<And>i. 2 \<le> i \<Longrightarrow> i < u32 (int n) + 1 \<Longrightarrow> fact (unat i-1) < (2::int)^32 \<Longrightarrow> checked_mul (u32 (fact (unat i - Suc 0))) i = Some (u32 (fact (unat i)))"
+  apply (clarsimp simp: checked_mul word_mult_def uint_word_of_int int_mod_eq' unat_def)
+  apply safe
+   apply (subst 1)
+    apply uint_arith
+   apply simp
+  apply (subst 1)
+   apply uint_arith
+  apply (rule 3[unfolded unat_def]; simp)
+  done
+   
+  show ?thesis
+  apply simp
+  apply (rule loop_range_u32'[where P="\<lambda>i res. fact (unat i-1) < 2^32 \<and> res = u32 (fact (unat i-1))"])
+      apply (auto simp: examples_fac_4_def)[1]
+     apply (auto simp: bind_eq_Some_conv)[1]
+     apply (subst 2; simp)
+    apply (rule 3; simp)
+   apply (auto)[1]
+  sorry
+qed
 
 end
